matching-logic/src/ProofMode.v
@@ -131,6 +131,19 @@ Open Scope ml_scope.
 
   #[local] Hint Resolve wf_app : core.
 
+(* A proof together with some properties of it. *)
+Record ProofWithInfo {Σ : Signature} (Γ : Theory) (ϕ : Pattern) := mkNiceProof
+{
+  pwi_generalized_evars : EVarSet ;
+  pwi_substituted_svars : SVarSet ;
+  pwi_uses_kt : bool ;
+  pwi_pf : Γ ⊢ ϕ ;
+  
+  pwi_pf_ge : @uses_of_ex_gen Σ Γ ϕ pwi_pf ⊆ pwi_generalized_evars ;
+  pwi_pf_svs : @uses_of_svar_subst Σ Γ ϕ pwi_pf ⊆ pwi_substituted_svars ;
+  pwi_pf_kt : implb (@uses_kt Σ Γ ϕ pwi_pf) pwi_uses_kt ;
+}.
+
 
 Record MyGoal {Σ : Signature} : Type := mkMyGoal { mgTheory : Theory; mgHypotheses: list Pattern; mgConclusion : Pattern }.
 
@@ -703,8 +716,15 @@ Section FOL_helpers.
         * eapply (P1 _ ((B ---> C) ---> B ---> D) A _ _).
       + eapply (P2 _ A (B ---> C) (B ---> D) _ _ _).
         Unshelve.
-        all: auto 10.
+        all: wf_auto2.
   Defined.
+
+  (* I would like the lemmas proved using tactics, and other lemmas too,
+    to carry with them an information about
+     what evars they generalize on.
+     There will be a record for it, together with a coercion/projection of the proof itself.
+     There will be a variant of Deduction theorem that takes the record as its input.
+   *)
 
   Lemma syllogism_4_meta_indifferent
         P {Pip : IndifProp P} Γ a b c d
@@ -883,6 +903,7 @@ Section FOL_helpers.
         P {Pip : IndifProp P} Γ a (wfa : well_formed a = true)
     := ProofProperty0 P _ (@not_not_elim_indifferent P _ Γ _ wfa).
 
+    (* Now I think that MyGoal has to be aware *)
   Lemma not_not_elim_meta Γ A :
     well_formed A ->
     Γ ⊢ (! ! A) ->
